BDL.lean
@@ -1,8 +1,8 @@
 import BDL.Core.Base
-import BDL.Core.Spec
-import BDL.Core.Hole
+import BDL.Core.Interface
+import BDL.Core.Decl
 import BDL.Core.Typing
 import BDL.Core.Satisfaction
 import BDL.Core.Env
 import BDL.Core.Dependency
-import BDL.Experiments.HoleCounterexamples
+import BDL.Experiments.DeclCounterexamples
